---
layout: default
---

## Algebra Foundations

### Exponents

<div class="math">
<p>
 \( 8^{3} \),  \( 3^{4} \),  \( 4^{8} \)
</p>
 <p>
 \( (\frac{1}{5})^{3} \) = \( \frac{1}{5} \times \frac{1}{5} \times \frac{1}{5} \) = \( \frac{1}{125} \)
</p>
</div>

#### Exponent Properties
1. Multiply Powers

  <div class="math">
  <p>
  (\( 8^{3})^{4} \) = \( 8^{12} \)
  </p>
  <p>
  \( (5^{3})^{2} \) = \( 5^{6} \)
  </p>
  <p>
  \( {5}({4x} + {3y} - {6}) \) = \( {5}({4x}) + {5}({3y}) - {5}({6}) = {20x} + {15y} - {30}  \)
  </p> 
  <p>
  \( ({x^2} + {1}) ({y} - {2}) \) = \( {x^2}({y} - {2}) + 1 ({y} - {2}) \) = \( {y}{x^2} - {2}{x^2} + {y} - {2} \)
  </p>  
  </div>
  
2. Divide Powers

  <div class="math">
  <p>
  \( \frac{4^6}{4^x} = 4^{6} \div 4^{x} = 4^{6-x} \)
  </p>
  <p>
  \(\frac{a^6}{a} = a^{6} \div a^{1} = a^{6 - 1} = a^{5}\)
  </p>
  </div>
  
3. Powers of Products and Quotients

  <div class="math">
  <p>
  \( (3 \times 6)^3 \) = \( 3^{3} \times 6^{3} \) = \( 3^{3} \times 6^{3} \)
  </p>
  <p>
  (\(8^{3})^{4}\) = \( 8^{12} \)
  </p>
  </div>  
  
4. Multiply Powers of the same base

  <div class="math">
  <p>
  \( 2^{3} \times 2^{4} \) = \( 2^{3 + 4} \)
  </p>
  </div>
  
5. Power of zero = 1

  <div class="math">
  <p>
  \( \frac{4^6}{4^6} = 4^{6} \div 4^{6} = 4^{6-6} = 4^{0} = 1 \)
  </p>
  </div>

5. Negative Exponents

  <div class="math">
  <p>
  \( {10}^{-14} = \frac{1}{10^14} \)
  </p>
   <p>
  \( \frac{1}{x^a} = {x^-a} \)
  </p>
  <p>
  \( {2^-3} = \frac{1}{2^3} = \frac{1}{2} \times \frac{1}{2} \times \frac{1}{2} = \frac{1}{8}\)
  </p>
  </div>
  
6. Complex Functions

  <div class="math">
  <p>
  \( {10}^{-14} = \frac{1}{10^14} \)
  </p>
  <p>
  \( \frac{1}{\frac{1}{3^4}} = {1} \div \frac{1}{3^4} = {1} \times \frac{3^4}{1} = {3^4} \)
  </p>
  <p>
  \( {2^-3} = \frac{1}{2^3} = \frac{1}{2} \times \frac{1}{2} \times \frac{1}{2} = \frac{1}{8}\)
  </p>
  </div>
  
7. Square Roots

  <div class="math">
  <p>
  \( \sqrt{a} = {b} \)  which means \( {b^2} = {a} \)
  </p>
  <p> <b>Addition and subtraction</b> </p>
  <p>
  \( {m}\sqrt{a} + {n}\sqrt{a} = ({m} + {n})\sqrt{a} \)
  </p>
  <p>
  \( {m}\sqrt{a} - {n}\sqrt{a} = ({m} - {n})\sqrt{a} \)
  </p> 
  <p> <b>Absolute Values</b> </p>
  <p>
  \( \sqrt{a} \times \sqrt{a} = \sqrt{a^2} = |a| \)
  </p>
  <p> <b>Multiplication</b> </p>
  <p>
  \( \sqrt{a} \times \sqrt{b} = \sqrt{ab} \)
  </p> 
  <p> <b>Division</b> </p>
  <p>
  \( \frac{\sqrt{a}}{\sqrt{b}} = \sqrt{\frac{a}{b}} \)
  </p>  
  <p> <b>Radical Form to Fraction</b> </p>
  <p>
  \( \sqrt[3]{a} = {a}^\frac{1}{3} \)
  </p>   
  <p>
  \( \sqrt[3]{a^2} = {a}^\frac{2}{3} \)
  </p>    
  </div>
  
#### Methods used in Algebra
##### Factoring methods

  <div class="math">
  <p> <b>Factoring Letters</b> </p>
  <p>
  \( {a}{b} + {a}{c} + {a}{d} = {a}({b} + {C} + {d})\)
  </p>
  <p> <b>Factoring Numbers</b> </p>
  <p>
  \( {12}{x^2}{y^3}{z} + {18}{x^3}{y^2}{z^2} - {24}{x}{y^4}{z^3} = {6}{x^2}{y^2}{z}({2}{y}{z} + {3}{x}{z} - {4}{y^2}{z^2}) \)
  </p> 
  </div>  
  
##### FOIL methods
Quadratic equations are formed from multiplying two binomials or expressions.

Example 1:
<div class="math">
<p> <b>Factoring Letters</b> </p>
<p>
  \( {6}{x^2} + {7x} - {3} \)
</p>
<p>
<p> <b>First (F): Product of the first terms</b> </p>
   \( {2x} \times {3x} = {6}{x^2} \)
</p>
<p> <b>Outer (O): Product of the outer terms</b> </p>
  \( {-1} \times {3} = {-3} \)
  
<p> <b>Inner (I): Product of the inner terms</b> </p> 
  
  \( ({2} \times {-1}) + ({3} \times {3}) = {-2} + {9} = {7} \)
  
<p> <b>Last (L): Product of the last terms</b> </p>
  \( {-3} \)
  
<p> <b>Answer: \( ({2x} - {3}) ({3x} - {1}) \) </b> </p>
    
</div>  
  
Example 2:
<div class="math">
<p> <b>Factoring Letters</b> </p>
<p>
  \( {2}{x^2} + {5x} - {12} \)
</p>
<p>
<p> <b>First (F): Product of the first term</b> </p>
   \( {2x} \times {1x} = {2}{x^2} \)
</p>
<p> <b>Outer (O): Product of the outer term</b> </p>
  \( {4} \times {-3} = {5} \)  #Get the multiple that when added will equal +5
  
<p> <b>Inner (I): Product of the inner term</b> </p> 
  
  \( ({2} \times {4}) + ({1} \times {-3}) = {8} + {-3} = {5} \)
  
<p> <b>Last (L): Product of the last term</b> </p>
  \( {-12} \)
  
<p> <b>Answer: \( ({2x} - {3}) ({1x} + {4}) \) </b> </p>
</div>  
